\documentclass{article}


\begin{document}
\title{CNF Grammar of our language}
\author{Mobin Razavi, Ali Ahmadvand, Mohammad Davoodabadi}
\date{}
\maketitle
Our grammar is based on C-minus grammar which you can find in \href{http://www.csci-snc.com/resources/ExamplesX/C-Syntax.pdf}{here}.
\begin{enumerate}
    \item program $\rightarrow$ declaration-list
    \item declaration-list $\rightarrow$ declaration-list   declaration $|$ declaration
    \item declaration $\rightarrow$ var-declaration $|$ fun-declaration
    \item var-declaration $\rightarrow$ type-spec ID; $|$ type-spec ID [NUM];
    \item type-spec $\rightarrow$ int $|$ float $|$ string
    \item fun-declaration $\rightarrow$ type-spec ID (params) compound-stmnt
    \item params $\rightarrow$ param-list $|$ $\epsilon$ 
    \item param-list $\rightarrow$ param-list, param $|$ param
    \item param $\rightarrow$ type-spec ID $|$ type-spec ID [ ]
    \item compound-stmnt $\rightarrow$ $\{$stmnt-list$\}$
    \item stmnt-list $\rightarrow$ stmnt-list stmnt $|$ $\epsilon$
    \item stmnt $\rightarrow$ compound-stmnt $|$ cond-stmnt $|$ iter-stmnt $|$ return-stmnt $|$ expression-stmnt $|$ var-declaration
    \item cond-stmnt $\rightarrow$ if (expression) stmnt  $|$ if (expression) compound-stmnt else compound-stmnt
    \item iter-stmnt $\rightarrow$ while (expression) compound-stmnt
    \item return-stmnt $\rightarrow$ return; $|$ return expression;
    \item expression-stmnt $\rightarrow$ expression; $|$ ;
    \item expression $\rightarrow$ var = expression $|$ simple-expression
    \item var $\rightarrow$ ID $|$ ID [expression]
    \item simple-expression $\rightarrow$ logical-expression rel-op logical-expression $|$ logical-expression
    \item rel-op $\rightarrow$ $>$ $|$ $<$ $|$ $>=$ $|$ $<=$ $|$ $==$ $|$ $!=$
    \item logical-expression $\rightarrow$ logical-expression log-op additive-expression $|$ additive-expression
    \item log-op $\rightarrow$ \&\& $|$ $||$
    \item additive-expression $\rightarrow$ additive-expression add-op mul-expression $|$ mul-expression
    \item add-op $\rightarrow$ $+$ $|$ $-$
    \item mul-expression $\rightarrow$ mul-expression mul-op term $|$ term
    \item mul-op $\rightarrow$ $*$ $|$ $/$
    \item term $\rightarrow$ (expression) $|$ var $|$ call $|$ NUM $|$ FNUM $|$ string-word
    \item call $\rightarrow$ ID (args) $|$ print(print-full-args)
    \item print-full-args $\rightarrow$ string args
    \item args $\rightarrow$ arg-list $|$ $\epsilon$
    \item arg-list $\rightarrow$ arg-list, expression $|$ expression
\end{enumerate}

keywords: if else int float string return while print \newline
Special symbols: $+ - *$ $/$ \& $|$ $>$ $<$ $>=$ $<=$ $==$ $!=$ $,$ $;$\newline
ID = $letter$ $(letter + digit)^*$ \newline
NUM = $digit^+$ \newline
FNUM = NUM.NUM \newline
string-word = "$(letter + digit + whitespace)^*$"






\end{document}
